\documentclass[a4paper,11pt]{article}
\usepackage{geometry}
 \geometry{
 a4paper,
 total={170mm,257mm},
 left=20mm,
 top=20mm,
 }
\usepackage{hyperref}
\usepackage{amsmath, amsfonts, amsthm, bbm}
\usepackage{cancel, color}
\renewcommand{\d}{{\mathrm{d}}}
\newcommand{\R}{{\mathrm{Ric}}}

\begin{document}
\noindent So let us define (in a proper basis)
\begin{align}
    A_{\mu\nu} :=& \nabla_\mu\nabla_\nu R&
    B_{\mu\nu} :=& \nabla_\rho\nabla^\rho R_{\mu\nu}.
\end{align}
And let us express their associated 2-tensors, using $X:=x^\mu e_\mu; Y:=y^\mu e_\mu;$ and $Z$ as dummy variables. We will use the notation $X\circ Y:= f \mapsto x^\mu \partial_\mu (y^\nu e_\nu f)$ for derivation along feilds.
\begin{align*}
    A(X,Y) :\!\!&= x^\mu y^\nu A_{\mu\nu}\\
    :\!\!&= x^\mu y^\nu \nabla_\mu \nabla_\nu R\\
    &= x^\mu y^\nu \nabla_\mu \partial_\nu R\\
    &= x^\mu y^\nu \partial_\mu \partial_\nu R - x^\mu y^\nu \Gamma_{\mu\nu}^\lambda \partial_\lambda R\\
    &= x^\mu \partial_\mu \left(y^\nu \partial_\nu R \right) - x^\mu \cdot(\partial_\mu y^\nu) \cdot (\partial_\nu R) - x^\mu y^\nu (\nabla_{e_\mu} \partial_\nu)R\\
    &= x^\mu \partial_\mu \left(y^\nu \partial_\nu R \right) - \cancel{x^\mu \cdot(\partial_\mu y^\nu) \cdot (\partial_\nu R)} - x^\mu \big(\nabla_{e_\mu} (y^\nu \partial_\nu)\big)R + \cancel{x^\mu \cdot (\partial_\mu y^\nu) \cdot (\partial_\nu R)}\\
    &= (X\circ Y - \nabla_X Y) R
\end{align*}
Thus:
\begin{equation}
    A : \Bigg\{\begin{matrix}
        T\mathcal{M}^{\otimes 2} & \to & \mathbb{R}\\
        (X,Y) & \mapsto & \frac{1}{2}\big(X\circ Y + Y\circ X - \nabla_X Y - \nabla_Y X\big) R
    \end{matrix}
\end{equation}
Now, although this derivation was rather easy to find, the case of $B$ is a lot more hard to get blindly. We will thus need to go a bit more subtly.
\\
First, let us acknowledge the fact that $B(X,Y)=\mathrm{tr}_g(Z\mapsto z^\rho z^\sigma x^\mu y^\mu \nabla_\rho \nabla_\sigma R_{\mu\nu})$. Which is already a bit scary. Next, we compute the tensorial (physics notation) expression
\begin{align*}
    \nabla_\rho \nabla_\sigma R_{\mu\nu} &=
    \partial_\rho \nabla_\sigma R_{\mu\nu}
    - \Gamma_{\rho\sigma}^\lambda \nabla_\lambda R_{\mu\nu}
    - \Gamma_{\rho\mu}^\lambda \nabla_\sigma R_{\lambda\nu}
    - \Gamma_{\rho\nu}^\lambda \nabla_\sigma R_{\mu\lambda}\\
    &=\partial_\rho \partial_\sigma R_{\mu\nu}
    - \partial_\rho\big( \Gamma_{\sigma\mu}^\lambda R_{\lambda\nu} \big)
    - \partial_\rho \big( \Gamma_{\sigma\nu}^\lambda R_{\mu\lambda} \big)
    - \Gamma_{\rho\sigma}^\lambda \partial_\lambda R_{\mu\nu}
    + \Gamma_{\rho\sigma}^\lambda \Gamma_{\lambda\mu}^\delta R_{\delta\nu}
    + \Gamma_{\rho\sigma}^\lambda \Gamma_{\lambda\nu}^\delta R_{\mu\delta}\\
    &\quad- \Gamma_{\rho\mu}^\lambda \partial_\sigma R_{\lambda\nu}
    + \Gamma_{\rho\mu}^\lambda \Gamma_{\sigma\lambda}^\delta R_{\delta\nu}
    + \Gamma_{\rho\mu}^\lambda \Gamma_{\sigma\nu}^\delta R_{\lambda\delta}
    - \Gamma_{\rho\nu}^\lambda \partial_\sigma R_{\mu\lambda}
    + \Gamma_{\rho\nu}^\lambda \Gamma_{\sigma\mu}^\delta R_{\delta\lambda}
    + \Gamma_{\rho\nu}^\lambda \Gamma_{\sigma\lambda}^\delta R_{\mu\delta}\\
    &=\partial_\rho \partial_\sigma R_{\mu\nu}
    + \Gamma_{\rho\sigma}^\lambda \Gamma_{\lambda\mu}^\delta R_{\delta\nu}
    + \Gamma_{\rho\sigma}^\lambda \Gamma_{\lambda\nu}^\delta R_{\mu\delta}
    + \Gamma_{\rho\mu}^\lambda \Gamma_{\sigma\lambda}^\delta R_{\delta\nu}
    + \Gamma_{\rho\mu}^\lambda \Gamma_{\sigma\nu}^\delta R_{\lambda\delta}
    + \Gamma_{\rho\nu}^\lambda \Gamma_{\sigma\mu}^\delta R_{\delta\lambda}
    + \Gamma_{\rho\nu}^\lambda \Gamma_{\sigma\lambda}^\delta R_{\mu\delta}\\
    &\quad - \partial_\rho \Gamma_{\sigma\mu}^\lambda R_{\lambda\nu}
    - \partial_\rho \Gamma_{\sigma\nu}^\lambda R_{\mu\lambda}
    - \Gamma_{\sigma\mu}^\lambda \partial_\rho R_{\lambda\nu}
    - \Gamma_{\sigma\nu}^\lambda \partial_\rho R_{\mu\lambda}
    - \Gamma_{\rho\sigma}^\lambda \partial_\lambda R_{\mu\nu}
    - \Gamma_{\rho\mu}^\lambda \partial_\sigma R_{\lambda\nu}
    - \Gamma_{\rho\nu}^\lambda \partial_\sigma R_{\mu\lambda}
\end{align*}
From here, it seems still far too hard to factorize elements into nice mathematical expressions like we did for $A$, so instead, we shall first attempt educated guesses for $D(X,Y,Z,Z)=z^\rho z^\sigma x^\mu y^\mu \nabla_\rho \nabla_\sigma R_{\mu\nu}$.

A candid reader would probably think of $D(X,Y,Z,Z)=\nabla_Z \nabla_Z \R(X,Y)$ by a simple symbol-to-symbol identification. Although this guess is incorrect, it puts us on the right path: \emph{it fails because it is not a tensor}.

Indeed recal that a tensor $D(X,Y,Z,...)$ must be linear in all its parameters. Or (as these expressions will be used for computations steps) \emph{addition morphism} and \emph{scaling morphism}. Although the guess $D(X,Y,Z,Z)=\nabla_Z \nabla_Z \R(X,Y)$ is an addition morphism, one can easily check it is no scale morphism:
\begin{align*}
\nabla_Z \nabla_Z \R(\lambda X,Y)
    &=\nabla_Z \nabla_Z\big( \lambda \R(X,Y) \big)\\
    &= \nabla_Z \big(\lambda\nabla_Z \R(X,Y) \big)
    + \nabla_Z \big( Z(\lambda) \cdot \R(X,Y) \big)\\
    &= \lambda \nabla_Z \nabla_Z \R(X,Y)
    + 2 \cdot Z(\lambda) \cdot \nabla_Z \R(X,Y)
    + \nabla_Z \big( Z(\lambda)\big) \cdot \R(X,Y)\\
    &\ne \lambda \nabla_Z \nabla_Z \R(X,Y)
\end{align*}
Also, note that $R(X,Y)$ is a scalar, thus $\nabla_Z\R(X,Y)=Z\big(\R(X,Y)\big)$.\\

We will thus attempt to compensate for it with other terms, as we know our true result must be a tensor anyway. To do so, we list all the addition morphism terms that use the same elements in a similar fashion\footnote{Note that we will use awkward self-made notations in order to shorten the formulae, without any explanation for their use. This is because, not only are they (to our mind) quite intuitive, they are also useless to understand as all of their uses is followed by the same expression without their use. They just happen to be infinietely more compact and thus a bit more readable.}. Here is the list of all such terms:

\begin{align*}
    \langle\langle \quad:\quad&\quad
    \R(\nabla_Z\nabla_Z X,\;Y)
    &\rangle\rangle \quad:\quad&\quad
    \R(X,\;\nabla_Z\nabla_ZY)\\
    \textcircled{$\langle$}\!\!\! \quad:\quad&\quad
    Z\big(\R(\nabla_Z X,\;Y)\big)
    &\textcircled{$\rangle$}\! \quad:\quad&\quad
    Z\big(\R( X,\;\nabla_ZY)\big)\\
    \langle\rangle \!\!\!\quad:\quad&\quad
    \R(\nabla_Z X, \nabla_Z Y)
    & \textcircled{$\circ$}\! \quad:\quad&\quad
    Z\big(Z\big(\R(X,Y)\big)\big)
\end{align*}
Before we start mixing them arround to get $X$ and $Y$ scaling, it is actually easier to add correcting terms to get the correct quadratic in $Z$ behavior as folows:
\begin{align*}
    \langle\langle \quad:\quad&\quad
    \R\big((\nabla_Z\nabla_Z-\nabla_{\nabla_Z Z}) X,\;Y\big)
    &\rangle\rangle \quad:\quad&\quad
    \R\big(X,\;(\nabla_Z\nabla_Z-\nabla_{\nabla_Z Z})Y\big)\\
    \textcircled{$\langle$}\!\!\! \quad:\quad&\quad
    Z\big(\R(\nabla_Z X,\;Y)\big) - \R\big(\nabla_{\nabla_ZZ}X,Y\big)
    &\textcircled{$\rangle$}\! \quad:\quad&\quad
    Z\big(\R( X,\;\nabla_ZY)\big)- \R\big(X,\nabla_{\nabla_ZZ}Y\big)\\
    \langle\rangle \!\!\!\quad:\quad&\quad
    \R(\nabla_Z X, \nabla_Z Y)
    & \textcircled{$\circ$}\! \quad:\quad&\quad
    \big(\nabla_Z\nabla_Z-\nabla_{\nabla_Z Z}\big)\R(X,Y)
\end{align*}
We let the courageous readers verify that for given $X$, $Y$ these expressions are all tensors in $Z$ and $Z$ and we go straight to seeing how they behave under scaling of $X$.
\begin{align*}
    \langle\langle \quad:&&
    \R(\nabla_Z\nabla_Z \lambda X,\;Y)
    &= \R\big(\nabla_Z(\lambda\nabla_Z  X),\;Y\big) + \R\big(\nabla_Z (Z(\lambda) X),\;Y\big)\\
    &&&= \lambda\R(\nabla_Z\nabla_Z  X,\;Y) + 2 Z(\lambda)\R(\nabla_Z  X,\;Y) + Z^2(\lambda) \R(X,Y)\\
    &&\R(\nabla_{\nabla_ZZ}\lambda X,Y)
    &= \lambda \R(\nabla_{\nabla_ZZ}X,Y) + \nabla_{\nabla_ZZ}(\lambda)\R(X,Y)\\
    &&\R\big((\nabla_Z\nabla_Z-\nabla_{\nabla_ZZ})\lambda X,Y\big)
    &= \lambda \R\big((\nabla_Z\nabla_Z-\nabla_{\nabla_ZZ}) X,Y\big) + 2 Z(\lambda)\R(\nabla_Z  X,\;Y) 
    \\&&&\quad + \big(Z^2(\lambda)- \nabla_{\nabla_ZZ}(\lambda)\big)\R(X,Y)\\
    \rangle\rangle \;\;:&& 
    \R\big((\lambda X,\;(\nabla_Z\nabla_Z-\nabla_{\nabla_ZZ})Y\big))
    &= \lambda \R\big((X,\;(\nabla_Z\nabla_Z-\nabla_{\nabla_ZZ})Y\big))\\
    \textcircled{$\langle$} \;\,:&&
    Z\big(\R(\nabla_Z \lambda X,\;Y)\big) - \R(\nabla_{\nabla_ZZ}\lambda X,Y)
    &= Z\big(\lambda\R(\nabla_Z X,\;Y)\big)
    + Z\big(Z(\lambda) \cdot \R(X,\;Y)\big)\\
    &&&\quad - \lambda \R(\nabla_{\nabla_ZZ}X,Y) - \nabla_{\nabla_ZZ}(\lambda)\R(X,Y)\\
    &&&= \lambda \Big(Z\big(\R(\nabla_Z X,Y)\big)-
    \R(\nabla_{\nabla_ZZ}X,Y) \Big)+ Z(\lambda) \R(\nabla_Z X, Y)\\
    &&&\quad + Z(\lambda) Z\big(\R(X,Y)\big) + \big(Z^2(\lambda) - \nabla_{\nabla_ZZ}(\lambda)\big)\R(X,Y) \\
    \textcircled{$\rangle$} \;\,:&&
    Z\big(\R(\lambda X,\;\nabla_ZY)\big)- \R(\lambda X,\nabla_{\nabla_ZZ}Y)
    &= \lambda \Big(Z\big(\R(X,\;\nabla_ZY)\big)- \R(X,\nabla_{\nabla_ZZ}Y)\Big)
    + Z(\lambda)\R(X,\;\nabla_ZY)\\
    \langle\rangle \;\;:&&
    \R(\nabla_Z \lambda X, \; \nabla_Z Y)
    &= \lambda \R(\nabla_Z X, \; \nabla_Z Y)
    + Z(\lambda) \R(X,\; \nabla_Z Y)\\
    \textcircled{$\circ$} \;\,:&&
    Z^2\big(\R(\lambda X,\;Y)\big) &= \lambda Z^2\big(\R( X,\;Y)\big)
    + 2 Z(\lambda) Z\big(\R(X,Y)\big)
    + Z^2(\lambda) \R(X,Y)\\
    &&\nabla_{\nabla_ZZ}\big(\R(\lambda X,Y)\big)
    &=\lambda\nabla_{\nabla_ZZ}\big(\R( X,Y)\big)
    + \nabla_{\nabla_ZZ}(\lambda)\R(X,Y)\\
    && \big(\nabla_Z\nabla_Z-\nabla_{\nabla_Z Z}\big)\R(\lambda X,Y)
    &= \lambda \big(\nabla_Z\nabla_Z-\nabla_{\nabla_Z Z}\big)\R(X,Y) + 2 Z(\lambda) Z\big(\R(X,Y)\big)\\
    &&&\quad + \big(Z^2(\lambda)-\nabla_{\nabla_ZZ}(\lambda)\big) \R(X,Y)
\end{align*}
From these transformations, (or the diagram here-under) it is trivial to find all possible tensors.
\begin{equation}
\boxed{\quad \begin{matrix}
    \quad\\
    \langle\langle & \mapsto  & \lambda\; \langle\langle & + & 2 \; \langle & + & \cdot \\
    \rangle\rangle & \mapsto & \lambda\; \rangle\rangle \\
    \textcircled{$\langle$} & \mapsto & \lambda\; \textcircled{$\langle$} & + & \langle & + & \circ & + & \cdot \\
    \textcircled{$\rangle$} & \mapsto & \lambda\; \textcircled{$\rangle$} & + & \rangle  \\
    \langle\rangle & \mapsto & \lambda\; \langle\rangle & + & \rangle \\
    \textcircled{$\circ$} & \mapsto & \lambda\; \textcircled{$\circ$} & + & 2 \; \circ & + & \cdot\\
    \quad
\end{matrix}\quad }
\end{equation}
One trivially finds (by starting from any of the guesses, compensating terms and keeping track of the symmetry of the tensor with respect to $X$ and $Y$) that the only possible linear combination that leads to a scale morphism is $\langle\langle \; + \;\rangle\rangle+\textcircled{$\circ$} + 2 \langle\rangle - 2 \textcircled{$\langle$}- 2 \textcircled{$\rangle$}$, or in proper words $D$ can only be, up to scale factors:
\begin{align*}
    D(X,Y,Z,Z) &= \R\big((\nabla_Z\nabla_Z-\nabla_{\nabla_Z Z}) X,\;Y\big)
    + \R\big( X,\;(\nabla_Z\nabla_Z-\nabla_{\nabla_Z Z})Y\big)
    + \big(\nabla_Z\nabla_Z-\nabla_{\nabla_Z Z}\big)\R(X,Y)\\
    & \quad -2 Z\big(\R(\nabla_Z X, Y)\big)
    +2 \R(\nabla_{\nabla_ZZ} X,Y) 
    -2 Z\big(\R(X, \nabla_Z Y)\big)
    +2 \R( X,\nabla_{\nabla_ZZ}Y) \\
    & \quad + 2 \R(\nabla_Z X, \nabla_Z Y)\\
    &=\R(\nabla_Z\nabla_Z X,Y)
    + \R( X,\nabla_Z\nabla_ZY)
    + \R(\nabla_{\nabla_ZZ} X,Y)
    + \R( X,\nabla_{\nabla_ZZ}Y)\\
    & \quad + Z\big(Z\big(\R(X,Y)\big)\big)-(\nabla_Z Z)\R(X,Y)
    -2 Z\big(\R(\nabla_Z X, Y)\big)
    -2 Z\big(\R(X, \nabla_Z Y)\big) \\
    & \quad + 2 \R(\nabla_Z X, \nabla_Z Y) 
\end{align*}
Let us compute each term seperately. Since we know the whole expression to be linear in $X$ and $Y$, and quadratic in $Z$ we can just evaluate them in $X=e_\mu,Y=e_\nu$, have one $Z$ be $e_\rho$ while the other is $e_\sigma$ and factorize the whole final expression with the scalar coordinate quantity $x^\mu y^\nu z^\rho z^\sigma$.
\begin{align*}
    \langle\langle \quad:\;
    \R\big((\nabla_{e_\rho}\nabla_{e_\sigma} - \nabla_{\nabla_{e_\rho}e_\sigma})e_\mu,\;e_\nu\big)
    &= \R\big(\nabla_{e_\rho}\Gamma_{\sigma\mu}^\lambda e_\lambda,e_\nu\big) - \Gamma_{\rho\sigma}^\lambda \R(\nabla_{e_\lambda}e_\mu,e_\nu)\\
    &=\Gamma_{\sigma\mu}^\lambda\R\big(\nabla_{e_\rho} e_\lambda,e_\nu\big) + \partial_\rho\Gamma_{\sigma\mu}^\lambda\R\big( e_\lambda,e_\nu\big)- \Gamma_{\rho\sigma}^\lambda \Gamma_{\lambda\mu}^\delta\R(e_\delta,e_\nu)\\
    &=\Gamma_{\sigma\mu}^\lambda\Gamma_{\rho\lambda}^\delta R_{\delta\nu} + \partial_\rho\Gamma_{\sigma\mu}^\lambda R_{\lambda\nu}- \Gamma_{\rho\sigma}^\lambda \Gamma_{\lambda\mu}^\delta R_{\delta\nu}\\
    \rangle\rangle \;\;:\;
    \R\big( e_\mu,\;(\nabla_{e_\rho}\nabla_{e_\sigma} - \nabla_{\nabla_{e_\rho}e_\sigma})e_\nu\big)
    &= \Gamma_{\sigma\nu}^\lambda \Gamma_{\rho\lambda}^\delta R_{\mu\delta} + \partial_\rho  \Gamma_{\sigma\nu}^\lambda R_{\mu\lambda}- \Gamma_{\rho\sigma}^\lambda \Gamma_{\lambda\nu}^\delta R_{\mu\delta}
\end{align*}
\begin{align*}
    \textcircled{$\langle$}\;\;: \; e_\rho\big(\R(\nabla_{e_\sigma} e_\mu, e_\nu)\big) - \R(\nabla_{\nabla_{e_\rho}e_\sigma} e_\mu, e_\nu)
    &= \partial_\rho (\Gamma_{\sigma\mu}^\lambda R_{\lambda\nu}) - \Gamma_{\rho\sigma}^\lambda \R(\nabla_{e_\lambda}e_\mu,e_\nu)\\
    &= \partial_\rho \Gamma_{\sigma\mu}^\lambda R_{\lambda\nu} + \Gamma_{\sigma\mu}^\lambda \partial_\rho R_{\lambda\nu} - \Gamma_{\rho\sigma}^\lambda \Gamma_{\lambda\mu}^\delta R_{\delta\nu}\\
    \textcircled{$\rangle$}\;\;: \; e_\rho\big(\R(e_\mu, \nabla_{e_\sigma} e_\nu)\big) - \R(e_\mu, \nabla_{\nabla_{e_\rho}e_\sigma} e_\nu)
    &= \partial_\rho \Gamma_{\sigma\nu}^\lambda R_{\mu\lambda} + \Gamma_{\sigma\nu}^\lambda \partial_\rho R_{\mu\lambda} - \Gamma_{\rho\sigma}^\lambda \Gamma_{\lambda\nu}^\delta R_{\mu\delta}
\end{align*}
\begin{align*}
\langle\rangle \quad:\;
    \R(\nabla_{e_\rho} e_\mu,\;\nabla_{e_\sigma} e_\nu)
    = \Gamma_{\rho\mu}^\lambda\Gamma_{\sigma\nu}^\delta R_{\lambda\delta}
\end{align*}
\begin{align*}
    \textcircled{$\circ$}\;\;: \; e_\rho\Big(e_\sigma\big(\R(e_\mu, e_\nu)\big)\Big) - (\nabla_{e_\rho}e_\sigma)\R(e_\mu,e_\nu)
    = \partial_\rho\partial_\sigma R_{\mu\nu} - \Gamma_{\rho\sigma}^\lambda \partial_\lambda R_{\mu\nu}
\end{align*}
This allows us to compute $D$, using $D(X,Y,Z,Z)=x^\mu y^\nu z^\rho z^\sigma D(e_\mu, e_\nu, e_\rho, e_\sigma =: x^\mu y^\nu z^\rho z^\sigma D_{\mu\nu\rho\sigma}$
\begin{align*}
D_{\mu\nu\rho\sigma} &= \Gamma_{\sigma\mu}^\lambda\Gamma_{\rho\lambda}^\delta R_{\delta\nu}
    + \partial_\rho\Gamma_{\sigma\mu}^\lambda R_{\lambda\nu}
    - \Gamma_{\rho\sigma}^\lambda \Gamma_{\lambda\mu}^\delta R_{\delta\nu}
    + \Gamma_{\sigma\nu}^\lambda \Gamma_{\rho\lambda}^\delta R_{\mu\delta}
    + \partial_\rho  \Gamma_{\sigma\nu}^\lambda R_{\mu\lambda}
    - \Gamma_{\rho\sigma}^\lambda \Gamma_{\lambda\nu}^\delta R_{\mu\delta}
    + 2 \Big(\Gamma_{\rho\mu}^\lambda\Gamma_{\sigma\nu}^\delta R_{\lambda\delta}\Big)\\
    &\quad -2\Big( \partial_\rho \Gamma_{\sigma\mu}^\lambda R_{\lambda\nu} + \Gamma_{\sigma\mu}^\lambda \partial_\rho R_{\lambda\nu} - \Gamma_{\rho\sigma}^\lambda \Gamma_{\lambda\mu}^\delta R_{\delta\nu}\Big)
    -2 \Big(\partial_\rho \Gamma_{\sigma\nu}^\lambda R_{\mu\lambda}
    + \Gamma_{\sigma\nu}^\lambda \partial_\rho R_{\mu\lambda}
    - \Gamma_{\rho\sigma}^\lambda \Gamma_{\lambda\nu}^\delta R_{\mu\delta}\Big)\\
    &\quad  + \partial_\rho\partial_\sigma R_{\mu\nu}
    - \Gamma_{\rho\sigma}^\lambda \partial_\lambda R_{\mu\nu}\\
    &= \Gamma_{\sigma\mu}^\lambda\Gamma_{\rho\lambda}^\delta R_{\delta\nu}
    + \cancel{\partial_\rho\Gamma_{\sigma\mu}^\lambda R_{\lambda\nu}}
    - \cancel{\Gamma_{\rho\sigma}^\lambda \Gamma_{\lambda\mu}^\delta R_{\delta\nu}}
    + \Gamma_{\sigma\nu}^\lambda \Gamma_{\rho\lambda}^\delta R_{\mu\delta}
    + \cancel{\partial_\rho  \Gamma_{\sigma\nu}^\lambda R_{\mu\lambda}}
    - \cancel{\Gamma_{\rho\sigma}^\lambda \Gamma_{\lambda\nu}^\delta R_{\mu\delta}}
    + 2 \Gamma_{\rho\mu}^\lambda\Gamma_{\sigma\nu}^\delta R_{\lambda\delta}\\
    &\quad -\cancel{2} \partial_\rho \Gamma_{\sigma\mu}^\lambda R_{\lambda\nu}
    -2 \Gamma_{\sigma\mu}^\lambda \partial_\rho R_{\lambda\nu}
    +\cancel{2} \Gamma_{\rho\sigma}^\lambda \Gamma_{\lambda\mu}^\delta R_{\delta\nu}
    -\cancel{2} \partial_\rho \Gamma_{\sigma\nu}^\lambda R_{\mu\lambda}
    -2 \Gamma_{\sigma\nu}^\lambda \partial_\rho R_{\mu\lambda}
    +\cancel{2} \Gamma_{\rho\sigma}^\lambda \Gamma_{\lambda\nu}^\delta R_{\mu\delta}\\
    &\quad  + \partial_\rho\partial_\sigma R_{\mu\nu}
    - \Gamma_{\rho\sigma}^\lambda \partial_\lambda R_{\mu\nu}\\
    &= \partial_\rho\partial_\sigma R_{\mu\nu}
    + \Gamma_{\rho\sigma}^\lambda \Gamma_{\lambda\mu}^\delta R_{\delta\nu}
    + \Gamma_{\rho\sigma}^\lambda \Gamma_{\lambda\nu}^\delta R_{\mu\delta}
    + \Gamma_{\sigma\mu}^\lambda\Gamma_{\rho\lambda}^\delta R_{\delta\nu}
    + \Gamma_{\rho\mu}^\lambda\Gamma_{\sigma\nu}^\delta R_{\lambda\delta}
    + \Gamma_{\rho\mu}^\lambda\Gamma_{\sigma\nu}^\delta R_{\lambda\delta}
    + \Gamma_{\sigma\nu}^\lambda \Gamma_{\rho\lambda}^\delta R_{\mu\delta}\\
    &\quad - \partial_\rho \Gamma_{\sigma\mu}^\lambda R_{\lambda\nu}
    - \partial_\rho \Gamma_{\sigma\nu}^\lambda R_{\mu\lambda}
    - \Gamma_{\sigma\mu}^\lambda \partial_\rho R_{\lambda\nu}
    - \Gamma_{\sigma\nu}^\lambda \partial_\rho R_{\mu\lambda}
    - \Gamma_{\rho\sigma}^\lambda \partial_\lambda R_{\mu\nu}
    - \Gamma_{\sigma\mu}^\lambda \partial_\rho R_{\lambda\nu}
    - \Gamma_{\sigma\nu}^\lambda \partial_\rho R_{\mu\lambda}\\
    &= \nabla_\rho \nabla_\sigma R_{\mu\nu}
\end{align*}
Thus:
\begin{equation}
    B:\bigg\{ \begin{matrix}
        T\mathcal{M}^{\otimes 2} & \to & \mathbb{R}\\
        (X,Y) & \mapsto & \mathrm{tr}_g \big(Z \mapsto D(X,Y,Z,Z)\big)
    \end{matrix}
\end{equation}

However ugly this is; it gives a formulation of $C=(2\alpha + \beta + 2\gamma) A +(4\gamma- \beta) B + \mathcal{O}(R^2)$ in a purely tensorial formulation (without a basis representation) through its image.

We can now split it back in our non-basis frame; and will, make extensive use of the properties we know about the connection to optimize our expressions as much as possible.

Firstly, as we already know we will contract $C_{\mu\nu}$ with a single null direction $l^\mu$, we know we only need to compute $C_{\pm\pm}$ in our frame.
This can be obtained by simply evaluating $C(X,Y)$ for $X=Y=\Sigma_i(0\cdot e_i) + 1 \cdot e_\pm + 0 \cdot e_\mp = e_\pm$ using bi-linearity of tensors. Indeed $C_{\pm\pm}:=C(e_\pm,e_\pm)$

\begin{align*}
    A_{\pm\pm} &= \partial_\pm \partial_\pm R - (\nabla_{e_\pm}e_\pm) R\\
    &= \partial_\pm \partial_\pm R - \underset{=0}{\cancel{\Gamma_{\pm\pm}^i}} \partial_i R - \Gamma_{\pm\pm}^\pm \partial_\pm R - \underset{=0}{\cancel{\Gamma_{\pm\pm}^\mp}} \partial_\mp R
\end{align*}
\begin{equation}
    \boxed{A_{\pm\pm} = \partial_\pm \partial_\pm R - \underset{\pm}{\omega}\partial_\pm R}
\end{equation}
\begin{align*}
    B_{\pm\pm}&= g^{\rho\sigma} D(e_\pm,e_\pm, e_\rho, e_\sigma)
\end{align*}
Recall \color{red} REF \color{black} the expression of $g^{-1}$:
$$g^{-1} = -(e_\pm \otimes e_\mp) - (e_\mp \otimes e_\pm) + g^{ij}e_i\otimes e_j $$
From this, one derives that 
$$B_{\pm\pm}=g^{ij}D(e_\pm,e_\pm, e_i, e_j) - D(e_\pm,e_\pm, e_\pm, e_\mp) - D(e_\pm,e_\pm, e_\mp, e_\pm) $$
Now, this will require $D(X,Y,Z,Z')$ to be defined for $Z\ne Z'$, which it is not, at the moment. But one can check by hand that the following generalization works flawlessly (and any generalisation will eventualy work, no need to symetrize it, as $B$'s formula treats $Z$ and $Z'$ the same):
\begin{align*}
    D(X,Y,Z,Z') 
    &=\R(\nabla_Z\nabla_{Z'} X ,Y )
    + \R( X ,\nabla_Z\nabla_{Z'} Y )
    + \R(\nabla_{\nabla_ZZ'} X , Y )
    + \R( X ,\nabla_{\nabla_ZZ'}Y )\\
    & \quad + Z\big(Z'\big(\R(X ,Y )\big)\big)-(\nabla_Z Z')\R(X ,Y )
    -2 Z\big(\R(\nabla_{Z'} X , Y )\big)
    -2 Z\big(\R(X , \nabla_{Z'} Y )\big) \\
    & \quad + 2 \R(\nabla_Z X , \nabla_{Z'} Y ) 
\end{align*} Thus \begin{align*}
    D(e_\pm,e_\pm,Z,Z') 
    &= 2 \R(\nabla_Z\nabla_{Z'} e_\pm ,e_\pm )
    + 2 \R(\nabla_{\nabla_ZZ'} e_\pm ,e_\pm )
    + Z\big(Z'\big(R_{\pm\pm}\big)\big)\\
    & \quad
    -(\nabla_Z Z') R_{\pm\pm}
    -4 Z\big(\R(\nabla_{Z'} e_\pm , e_\pm )\big)
    + 2 \R(\nabla_Z e_\pm , \nabla_{Z'} e_\pm )
\end{align*}
let us compute each term,
\begin{align*}
    D(e_\pm,e_\pm,e_i,e_j) 
    &= 2 \R(\nabla_{e_i}\nabla_{e_j} e_\pm ,e_\pm )
    + 2 \R(\nabla_{\nabla_{e_i}e_j} e_\pm ,e_\pm )
    + \partial_i \partial_j R_{\pm\pm}\\
    & \quad
    -(\nabla_{e_i} e_j) R_{\pm\pm}
    -4 \partial_i\big(\R(\nabla_{e_j} e_\pm , e_\pm )\big)
    + 2 \R(\nabla_{e_i} e_\pm , \nabla_{e_j} e_\pm )\\
    &= 2 \R\big(\nabla_{e_i}(\Gamma_{j\pm}^\mu e_\mu) ,e_\pm \big)
    -4 \partial_i(\Gamma_{j\pm}^\mu R_{\mu\pm})
    + 2 \Gamma_{j\pm}^\mu \R(\nabla_{e_i} e_\pm , e_\mu )\\
    & \quad
    + \partial_i \partial_j R_{\pm\pm}
    -\Gamma_{ij}^\mu \partial_\mu R_{\pm\pm}
    + 2 \Gamma_{ij}^\mu \R(\nabla_{e_\mu} e_\pm ,e_\pm )\\
    &= 2 \R\big(\nabla_{e_i}(\underset{\mp}{\chi}\,_{jl}g^{kl} e_k ) ,e_\pm \big)
    -4 \partial_i(\underset{\mp}{\chi}\,_{jl}g^{kl}  R_{k \pm})
    + 2 \underset{\mp}{\chi}\,_{jl}g^{kl}  \R(\nabla_{e_i} e_\pm , e_k  )\\
    &\quad
    \pm 2 \R\big(\nabla_{e_i}(\zeta_j e_\pm) ,e_\pm \big)
    \mp 4 \partial_i(\zeta_j R_{\pm\pm})
    \pm 2 \zeta_j \R(\nabla_{e_i} e_\pm , e_\pm )\\
    & \quad
    + \partial_i \partial_j R_{\pm\pm}
    -\Gamma_{ij}^k \partial_k R_{\pm\pm}
    + 2 \Gamma_{ij}^k \R(\nabla_{e_k} e_\pm ,e_\pm )\\
    & \quad
    -\underset{\pm}{\chi}\,_{ij} \partial_\pm R_{\pm\pm}
    -\underset{\mp}{\chi}\,_{ij} \partial_\mp R_{\pm\pm}
    + 2 \underset{\pm}{\chi}\,_{ij} \R(\nabla_{e_\pm} e_\pm ,e_\pm )
    + 2 \underset{\mp}{\chi}\,_{ij} \R(\nabla_{e_\mp} e_\pm ,e_\pm )\\
    &= 2 \partial_i(\underset{\mp}{\chi}\,_{jl}g^{kl}) R_{k\pm}
    + 2 \underset{\mp}{\chi}\,_{jl}g^{kl} \Gamma_{ik}^\mu R_{\mu\pm}
    -4 \partial_i(\underset{\mp}{\chi}\,_{jl}g^{kl})  R_{k \pm}
    -4 \underset{\mp}{\chi}\,_{jl}g^{kl}  \partial_i R_{k \pm}\\
    &\quad
    + 2 \underset{\mp}{\chi}\,_{jl}g^{kl} \Gamma_{i\pm}^\mu R_{\mu k}
    \pm 2 \zeta_j \Gamma_{i\pm}^\mu R_{\mu\pm}
    \pm 2 \partial_i \zeta_j R_{\pm\pm}
    \mp 4 \partial_i\zeta_j R_{\pm\pm}
    \mp 4 \zeta_j \partial_i R_{\pm\pm}\\
    & \quad
    \pm 2 \zeta_j \Gamma_{i\pm}^\mu R_{\mu\pm}
    + \partial_i \partial_j R_{\pm\pm}
    -\Gamma_{ij}^k \partial_k R_{\pm\pm}
    + 2 \Gamma_{ij}^k \Gamma_{k\pm}^\mu R_{\mu\pm}
    -\underset{\pm}{\chi}\,_{ij} \partial_\pm R_{\pm\pm}\\
    & \quad
    -\underset{\mp}{\chi}\,_{ij} \partial_\mp R_{\pm\pm}
    + 2 \underset{\pm}{\chi}\,_{ij} \Gamma_{\pm\pm}^\mu R_{\mu\pm}
    + 2 \underset{\mp}{\chi}\,_{ij} \Gamma_{\mp\pm}^\mu R_{\mu\pm}\\
    &= 2 \partial_i(\underset{\mp}{\chi}\,_{jl}g^{kl}) R_{k\pm}
    + 2 \underset{\mp}{\chi}\,_{jl}g^{lm} \Gamma_{im}^k R_{k\pm}
    + 2 \underset{\mp}{\chi}\,_{jl}g^{kl} \underset{\pm}{\chi}\,_{ik} R_{\pm\pm}
    + 2 \underset{\mp}{\chi}\,_{jl}g^{kl} \underset{\mp}{\chi}\,_{ik} R_{\mp\pm}\\
    &\quad
    - 4 \partial_i(\underset{\mp}{\chi}\,_{jl}g^{kl})  R_{k \pm}
    - 4 \underset{\mp}{\chi}\,_{jl}g^{kl}  \partial_i R_{k \pm}
    + 2 \underset{\mp}{\chi}\,_{jm}g^{km} \underset{\mp}{\chi}\,_{in}g^{nl} R_{kl}
    \pm 2 \underset{\mp}{\chi}\,_{jl}g^{kl} \zeta_i R_{k\pm}\\
    & \quad
    \pm 2 \zeta_j \underset{\mp}{\chi}\,_{il}g^{kl} R_{k\pm}
    + 2 \zeta_i \zeta_j R_{\pm\pm}
    \pm 2 \partial_i \zeta_j R_{\pm\pm}
    \mp 4 \partial_i\zeta_j R_{\pm\pm}
    \mp 4 \zeta_j \partial_i R_{\pm\pm}
    \pm 2 \zeta_j \underset{\mp}{\chi}\,_{il}g^{kl} R_{k\pm}\\
    & \quad
    + 2 \zeta_i \zeta_j R_{\pm\pm}
    + \partial_i \partial_j R_{\pm\pm}
    -\Gamma_{ij}^k \partial_k R_{\pm\pm}
    + 2 \Gamma_{ij}^l \underset{\mp}{\chi}\,_{lm}g^{km} R_{k\pm}
    \pm 2 \Gamma_{ij}^k \zeta_k R_{\pm\pm}\\
    &\quad 
    -\underset{\pm}{\chi}\,_{ij} \partial_\pm R_{\pm\pm}
    -\underset{\mp}{\chi}\,_{ij} \partial_\mp R_{\pm\pm}
    + 2 \underset{\pm}{\chi}\,_{ij} \underset{\mp}{\omega} R_{\pm\pm}
    + 2 \underset{\mp}{\chi}\,_{ij} \underset{\mp}{\eta}\,_l g^{kl} R_{k\pm}
    - 2 \underset{\mp}{\chi}\,_{ij} \underset{\pm}{\omega} R_{\pm\pm}\\
    &= 
    + 2 R_{\pm\pm} \Big( \underset{\pm}{\chi}\,_{ik} \underset{\mp}{\chi}\,_{jl}g^{kl}
    + \underset{\mp}{\omega} \underset{\pm}{\chi}\,_{ij}
    - \underset{\pm}{\omega} \underset{\mp}{\chi}\,_{ij}
    + 2 \zeta_i \zeta_j
    \pm \Gamma_{ij}^k \zeta_k 
    \mp \partial_i\zeta_j\Big)
    + 2 R_{kl} \underset{\mp}{\chi}\,_{in} \underset{\mp}{\chi}\,_{jm}g^{km}g^{nl}\\
    &\quad 
    + 2 R_{k\pm} \Big( \underset{\mp}{\chi}\,_{jl}g^{lm} \Gamma_{im}^k
    - \partial_i(\underset{\mp}{\chi}\,_{jl}g^{kl})
    + (\underset{\mp}{\chi}\,_{jl} \underset{\mp}{\chi}\,_{ik}
    + \underset{\mp}{\chi}\,_{ij} \underset{\mp}{\eta}\,_l
    \pm \zeta_i \underset{\mp}{\chi}\,_{jl}
    \pm 2 \zeta_j \underset{\mp}{\chi}\,_{il}
    + \Gamma_{ij}^m \underset{\mp}{\chi}\,_{ml} )g^{kl}\Big) \\
    &\quad 
    + 2 R_{\mp\pm} \underset{\mp}{\chi}\,_{jl} \underset{\mp}{\chi}\,_{ik} g^{kl}
    - 4 \underset{\mp}{\chi}\,_{jl}g^{kl}  \partial_i R_{k \pm}
    + \Big( \partial_i \partial_j
    \mp 4 \zeta_j \partial_i
    -\Gamma_{ij}^k \partial_k
    -\underset{\pm}{\chi}\,_{ij} \partial_\pm
    -\underset{\mp}{\chi}\,_{ij} \partial_\mp \Big) R_{\pm\pm}
\end{align*}


\begin{align*}
    \!\!\!\!\!\!\!\!\!\!\!\!\!\!\!
    D(e_\pm,e_\pm, e_\pm, e_\mp) 
    &=2 \R(\nabla_{e_\pm}\nabla_{{e_\mp}} e_\pm ,e_\pm )
    + 2 \R(\nabla_{\nabla_{e_\pm}{e_\mp}} e_\pm ,e_\pm )
    + \partial_\pm\partial_\mp R_{\pm\pm}
    -(\nabla_{e_\pm} {e_\mp})R_{\pm\pm}\\
    & \quad
    -4 \partial_\pm\big(\R(\nabla_{{e_\mp}} e_\pm , e_\pm )\big)
    + 2 \R(\nabla_{e_\pm} e_\pm , \nabla_{{e_\mp}} e_\pm )\\
    &=2 \R\big(\nabla_{e_\pm}(\Gamma_{\mp\pm}^\mu e_\mu) ,e_\pm \big)
    + 2 \Gamma_{\pm\mp}^\mu\R(\nabla_{e_\mu} e_\pm ,e_\pm )\\
    & \quad + \partial_\pm\partial_\mp R_{\pm\pm}
    -\Gamma_{\pm\mp}^\mu \partial_\mu R_{\pm\pm}
    -4 \partial_\pm\big(\Gamma_{\mp\pm}^\mu R_{\mu\pm}\big)
     + 2 \Gamma_{\mp\pm}^\mu \R(\nabla_{e_\pm} e_\pm , e_\mu ) \\
    &=2 \R\big(\nabla_{e_\pm}(\underset{\mp}{\eta}\,_j g^{ij} e_i) ,e_\pm \big)
    + 2 \underset{\pm}{\eta}\,_j g^{ij} \R(\nabla_{e_i } e_\pm ,e_\pm )\\
    & \quad + \partial_\pm\partial_\mp R_{\pm\pm}
    -\underset{\pm}{\eta}\,_j g^{ij}  \partial_i  R_{\pm\pm}
    -4 \partial_\pm\big(\underset{\mp}{\eta}\,_j g^{ij}  R_{i \pm}\big)
     + 2 \underset{\mp}{\eta}\,_j g^{ij}  \R(\nabla_{e_\pm} e_\pm , e_i  ) \\
    & \quad - 2 \R\big(\nabla_{e_\pm}(\underset{\mp}{\omega} e_\pm) ,e_\pm \big)
    - 2 \underset{\pm}{\omega}\R(\nabla_{e_\mp} e_\pm ,e_\pm )\\
    & \quad + \partial_\pm\partial_\mp R_{\pm\pm}
    +\underset{\pm}{\omega} \partial_\mp R_{\pm\pm}
    +4 \partial_\pm\big(\underset{\mp}{\omega} R_{\pm\pm}\big)
     - 2 \underset{\mp}{\omega} \R(\nabla_{e_\pm} e_\pm , e_\pm ) \\
    &=2 \underset{\mp}{\eta}\,_j g^{ij} \Gamma_{\pm i}^\mu R_{\mu\pm}
    + 2 \partial_\pm(\underset{\mp}{\eta}\,_j g^{ij}) R_{i\pm}
    + 2 \underset{\pm}{\eta}\,_j g^{ij} \Gamma_{i \pm}^\mu R_{\mu\pm}
    + \partial_\pm\partial_\mp R_{\pm\pm} 
    -\underset{\pm}{\eta}\,_j g^{ij}  \partial_i  R_{\pm\pm}
    -\underset{\pm}{\eta}\,_j g^{ij}  \partial_i  R_{\pm\pm}\\
    & \quad
    -4 \partial_\pm\big(\underset{\mp}{\eta}\,_j g^{ij} \big) R_{i \pm}
    -4 \underset{\mp}{\eta}\,_j g^{ij} \partial_\pm R_{i \pm}
     + 2 \underset{\mp}{\eta}\,_j g^{ij} \Gamma_{\pm\pm}^\mu R_{\mu i}
    - 2 \partial_\pm\underset{\mp}{\omega}  R_{\pm\pm}
    - 2 \underset{\mp}{\omega} \Gamma_{\pm\pm}^\mu R_{\mu\pm}
    - 2 \underset{\pm}{\omega}\Gamma_{\mp\pm}^\mu R_{\mu \pm}\\
    & \quad
    + \partial_\pm\partial_\mp R_{\pm\pm}
    +\underset{\pm}{\omega} \partial_\mp R_{\pm\pm}
    +4 \partial_\pm\big(\underset{\mp}{\omega} R_{\pm\pm}\big)
    - 2 \underset{\mp}{\omega} \Gamma_{\pm\pm}^\mu R_{\mu\pm}\\
    &=2 \underset{\mp}{\eta}\,_j g^{jk} \Gamma_{\pm k}^i R_{i\pm}
    + 2 \underset{\mp}{\eta}\,_j g^{ij} \Gamma_{\pm i}^\pm R_{\pm\pm}
    + 2 \partial_\pm(\underset{\mp}{\eta}\,_j g^{ij}) R_{i\pm}
    + 2 \underset{\pm}{\eta}\,_j g^{jk} \underset{_\mp}{\chi}\,_{kl}g^{il} R_{i\pm}
    \pm 2 \underset{\pm}{\eta}\,_j g^{ij} \zeta_i R_{\pm\pm}\\
    & \quad
    + \partial_\pm\partial_\mp R_{\pm\pm} 
    -\underset{\pm}{\eta}\,_j g^{ij}  \partial_i  R_{\pm\pm}
    -\underset{\pm}{\eta}\,_j g^{ij}  \partial_i  R_{\pm\pm}
    -4 \partial_\pm\big(\underset{\mp}{\eta}\,_j g^{ij} \big) R_{i \pm}
    -4 \underset{\mp}{\eta}\,_j g^{ij} \partial_\pm R_{i \pm}
     + 2 \underset{\mp}{\eta}\,_j g^{ij} \underset{\mp}{\omega}R_{\pm i}\\
    & \quad
    - 2 \partial_\pm\underset{\mp}{\omega}  R_{\pm\pm}
    - 2 \underset{\mp}{\omega} \underset{\mp}{\omega} R_{\pm\pm}
    - 2 \underset{\pm}{\omega}\underset{\mp}{\eta}\,_jg^{ij} R_{i \pm}
    + 2 \underset{\pm}{\omega}\underset{\pm}{\omega} R_{\pm \pm}
    + \partial_\pm\partial_\mp R_{\pm\pm}
    +\underset{\pm}{\omega} \partial_\mp R_{\pm\pm}
    +4 \partial_\pm\underset{\mp}{\omega} R_{\pm\pm} \\
    &\quad 
    + 4 \underset{\mp}{\omega} \partial_\pm R_{\pm\pm}
    - 2 \underset{\mp}{\omega}\underset{\mp}{\omega} R_{\pm\pm}\\
    &=
    2 R_{i \pm} \Big( \underset{\mp}{\eta}\,_j g^{jk} \Gamma_{\pm k}^i
    +  \underset{\pm}{\eta}\,_j \underset{_\mp}{\chi}\,_{kl} g^{jk} g^{il} 
    - \partial_\pm\big(\underset{\mp}{\eta}\,_j g^{ij} \big)
    + \underset{\mp}{\omega} \underset{\mp}{\eta}\,_j g^{ij}
    - \underset{\pm}{\omega} \underset{\mp}{\eta}\,_j g^{ij} \Big)
    -4 \underset{\mp}{\eta}\,_j g^{ij} \partial_\pm R_{i \pm}\\
    &\;\; 
    + 2 R_{\pm\pm} \Big(
    \underset{\pm}{\omega}\underset{\pm}{\omega}
    - 2 \underset{\mp}{\omega}\underset{\mp}{\omega}
    + \partial_\pm \underset{\mp}{\omega}
    + (\underset{\mp}{\eta}\,_{\!j} \underset{\pm}{\eta}\,_{\!i}
    \!\pm\! \underset{\pm}{\eta}\,_{\!j} \zeta_i )g^{ij} \!\Big)
    \!+\! \Big(\!2 \partial_\pm\partial_\mp
    +4 \underset{\mp}{\omega} \partial_\pm
    +\underset{\pm}{\omega} \partial_\mp
    -2\underset{\pm}{\eta}\,_{\!j}g^{ij}  \partial_i
    \Big) R_{\pm\pm}
\end{align*}

\begin{align*}
    D(e_\pm,e_\pm, e_\mp, e_\pm) 
    &=2\R(\nabla_{e_\mp}\nabla_{{e_\pm}} e_\pm ,e_\pm )
    + 2\R(\nabla_{\nabla_{e_\mp}{e_\pm}} e_\pm ,e_\pm )
    + \partial_\mp \partial_\pm R_{\pm\pm}
    -(\nabla_{e_\mp} {e_\pm})R_{\pm\pm}\\
    &\quad 
    -4 \partial_\mp\big(\R(\nabla_{{e_\pm}} e_\pm , e_\pm )\big)
    + 2 \R(\nabla_{e_\mp} e_\pm , \nabla_{{e_\pm}} e_\pm ) \\
    &=2\R\big(\nabla_{e_\mp}(\Gamma_{\pm\pm}^\pm e_\pm) ,e_\pm \big)
    + 2\Gamma_{\mp\pm}^\mu \R(\nabla_{e_\mu} e_\pm ,e_\pm )
    + \partial_\mp \partial_\pm R_{\pm\pm}
    -\Gamma_{\mp\pm}^\mu \partial_\mu R_{\pm\pm}\\
    &\quad 
    -4 \partial_\mp(\Gamma_{\pm\pm}^\pm R_{\pm\pm})
    + 2 \Gamma_{\pm\pm}^\pm \Gamma_{\mp\pm}^\mu R_{\mu\pm}\\
    &=2\underset{\mp}{\omega} \Gamma_{\mp\pm}^\mu R_{\mu\pm}
    + 2 \partial_\mp \underset{\mp}{\omega} R_{\pm\pm}
    + 2\Gamma_{\mp\pm}^\mu \R(\nabla_{e_\mu} e_\pm ,e_\pm )
    + \partial_\mp \partial_\pm R_{\pm\pm}
    -\Gamma_{\mp\pm}^\mu \partial_\mu R_{\pm\pm}\\
    &\quad 
    -4 \partial_\mp\underset{\mp}{\omega} R_{\pm\pm}
    -4 \underset{\mp}{\omega} \partial_\mp R_{\pm\pm}
    + 2 \underset{\mp}{\omega} \Gamma_{\mp\pm}^\mu R_{\mu\pm}\\
    &=2\underset{\mp}{\omega} \underset{\mp}{\eta}\,_j g^{ij} R_{i \pm}
    + 2 \partial_\mp \underset{\mp}{\omega} R_{\pm\pm}
    + 2\underset{\mp}{\eta}\,_k g^{jk} \underset{\mp}{\chi}\,_{jl}g^{il} R_{i\pm}
    \pm 2\underset{\mp}{\eta}\,_j g^{ij} \zeta_i R_{\pm\pm}
    + \partial_\mp \partial_\pm R_{\pm\pm}\\
    &\quad 
    -\underset{\mp}{\eta}\,_j g^{ij} \partial_i  R_{\pm\pm}
    -4 \partial_\mp\underset{\mp}{\omega} R_{\pm\pm}
    -4 \underset{\mp}{\omega} \partial_\mp R_{\pm\pm}
    + 2 \underset{\mp}{\omega} \underset{\mp}{\eta}\,_j g^{ij} R_{i \pm}\\
    &\quad - 2\underset{\mp}{\omega} \underset{\pm}{\omega} R_{\pm\pm}
    + 2 \partial_\mp \underset{\mp}{\omega} R_{\pm\pm}
    - 2\underset{\pm}{\omega} \underset{\pm}{\omega} R_{\pm\pm}
    + \partial_\mp \partial_\pm R_{\pm\pm}
    +\underset{\pm}{\omega} \partial_\pm R_{\pm\pm}\\
    &\quad 
    -4 \partial_\mp\underset{\mp}{\omega} R_{\pm\pm}
    -4 \underset{\mp}{\omega} \partial_\mp R_{\pm\pm}
    - 2 \underset{\mp}{\omega} \underset{\pm}{\omega} R_{\pm\pm}\\
    &= - 2 R_{\pm\pm} \Big(
    \mp \underset{\mp}{\eta}\,_j g^{ij} \zeta_i
    + 2 \underset{\mp}{\omega} \underset{\pm}{\omega}
    + \underset{\pm}{\omega} \underset{\pm}{\omega}
    +2 \partial_\mp\underset{\mp}{\omega} \Big)
    + 2 R_{i\pm} g^{ij} \Big(2 \underset{\mp}{\omega} \underset{\mp}{\eta}\,_j 
    + \underset{\mp}{\eta}\,_l \underset{\mp}{\chi}\,_{kj} g^{kl} \Big)\\
    &\quad
    + \Big(2 \partial_\mp \partial_\pm
    +\underset{\pm}{\omega} \partial_\pm
    -8 \underset{\mp}{\omega} \partial_\mp
    -\underset{\mp}{\eta}\,_j g^{ij} \partial_i  \Big) R_{\pm\pm}
\end{align*}
Summarizing, re-indexing and re-ordering...
\begin{align*}
    g^{ij} D(e_\pm,e_\pm,e_i,e_j)
    &= 
    + 2 R_{\pm\pm} \Big( \underset{\pm}{\chi}\,_{ik} \underset{\mp}{\chi}\,_{jl}g^{kl}g^{ij}
    + \underset{\mp}{\omega} \underset{\pm}{\chi}\,_{ij}g^{ij}
    - \underset{\pm}{\omega} \underset{\mp}{\chi}\,_{ij}g^{ij}
    + 2 \zeta_i \zeta_jg^{ij}
    \pm \Gamma_{ij}^k \zeta_k g^{ij}
    \mp g^{ij} \partial_i\zeta_j \Big)\\
    &\quad 
    + 2 R_{ij} \underset{\mp}{\chi}\,_{nm} \underset{\mp}{\chi}\,_{kl}g^{il}g^{jm}g^{kn} \\
    &\quad 
    + 2 R_{i\pm} \Big( \underset{\mp}{\chi}\,_{kl}\Gamma_{jm}^i g^{lm} g^{jk}
    \!-\! g^{jk} \partial_j(\underset{\mp}{\chi}\,_{kl}g^{il})
    \!+\! (\underset{\mp}{\chi}\,_{kl} \underset{\mp}{\chi}\,_{jk}
    \!+\! \underset{\mp}{\chi}\,_{jk} \underset{\mp}{\eta}\,_l
    \!\pm\! \zeta_j \underset{\mp}{\chi}\,_{kl}
    \!\pm\! 2 \zeta_k \underset{\mp}{\chi}\,_{jl}
    \!+\! \Gamma_{jk}^m \underset{\mp}{\chi}\,_{ml} )g^{il} g^{jk}\Big) \\
    &\quad 
    + 2 R_{\mp\pm} \underset{\mp}{\chi}\,_{jl} \underset{\mp}{\chi}\,_{ik} g^{kl} g^{ij}\\
    &\quad 
    - 4 \underset{\mp}{\chi}\,_{kl}g^{il}  g^{jk} \partial_j R_{i \pm}\\
    &\quad 
    +  \Big( g^{ij}\partial_i \partial_j
    \mp 4 \zeta_j g^{ij}\partial_i
    -\Gamma_{jk}^i g^{jk}\partial_i
    -\underset{\pm}{\chi}\,_{ij} g^{ij} \partial_\pm
    -\underset{\mp}{\chi}\,_{ij} g^{ij} \partial_\mp \Big) R_{\pm\pm}
\end{align*}

\begin{align*}
    \!\!\!\!\!\!\!\!\!\!
    - D_{\pm\pm\pm\mp} -D_{\pm\pm\mp\pm}
    &=
    + 2 R_{i \pm} \Big(
    + \partial_\pm\big(\underset{\mp}{\eta}\,_j g^{ij} \big)
    + \underset{\pm}{\omega} \underset{\mp}{\eta}\,_j g^{ij}
    -3 \underset{\mp}{\omega} \underset{\mp}{\eta}\,_j g^{ij}
    - \underset{\mp}{\eta}\,_j g^{jk} \Gamma_{\pm k}^i
    -  (\underset{\pm}{\eta}\,_l + \underset{\mp}{\eta}\,_l)  \underset{_\mp}{\chi}\,_{kj} g^{kl} g^{ij}  \Big)\\
    &\quad 
    +4 \underset{\mp}{\eta}\,_j g^{ij} \partial_\pm R_{i \pm}\\
    &\quad
    + 2 R_{\pm\pm} \Big(
    + 2 \underset{\mp}{\omega}\underset{\mp}{\omega}
    + 2 \underset{\mp}{\omega} \underset{\pm}{\omega}
    +2 \partial_\mp\underset{\mp}{\omega} 
    - \partial_\pm \underset{\mp}{\omega}
    - \underset{\pm}{\eta}\,_{i} \underset{\mp}{\eta}\,_{ j} g^{ij}  
     \mp  \zeta_i(\underset{\pm}{\eta}\,_{ j}+\underset{\mp}{\eta}\,_j)  g^{ij}\Big)\\
    &\quad 
    +  \Big(
    -2 \partial_\pm\partial_\mp
    -\underset{\pm}{\omega} \partial_\mp
    +8 \underset{\mp}{\omega} \partial_\mp
    -2 \partial_\mp \partial_\pm
    -4 \underset{\mp}{\omega} \partial_\pm
    -\underset{\pm}{\omega} \partial_\pm
    + (2\underset{\pm}{\eta}\,_{ j} + \underset{\mp}{\eta}\,_j) g^{ij}\partial_i
    \Big) R_{\pm\pm}
\end{align*}
Leads to the final expression:
\begin{align*}
    B_{\pm\pm} &= 
    + 2 R_{\pm\pm} \; \cdot \; \Big(
    + 2 \underset{\mp}{\omega}\underset{\mp}{\omega}
    + 2 \underset{\mp}{\omega} \underset{\pm}{\omega}
    +2 \partial_\mp\underset{\mp}{\omega} 
    - \partial_\pm \underset{\mp}{\omega}\\
     &\quad \quad \quad \quad \quad \quad \; \;
    + g^{ij} \big(2 \zeta_i \zeta_j
    - \underset{\pm}{\eta}\,_{i} \underset{\mp}{\eta}\,_{ j}
    \mp  \zeta_i(\underset{\pm}{\eta}\,_{ j}+\underset{\mp}{\eta}\,_j)
    + \underset{\pm}{\chi}\,_{ik} \underset{\mp}{\chi}\,_{jl}g^{kl}
    + \underset{\mp}{\omega} \underset{\pm}{\chi}\,_{ij}
    - \underset{\pm}{\omega} \underset{\mp}{\chi}\,_{ij}
    \pm \Gamma_{ij}^k \zeta_k 
    \mp \partial_i\zeta_j \big)
    \Big)\\
    &\quad 
    +  \Big(
    + g^{ij}\partial_i \partial_j
    -2 \partial_\pm\partial_\mp
    -2 \partial_\mp \partial_\pm
    -\Gamma_{jk}^i g^{jk}\partial_i
    + (2\underset{\pm}{\eta}\,_{ j} + \underset{\mp}{\eta}\,_j \mp 4 \zeta_j) g^{ij}\partial_i\\
    &\quad \quad \;\;\;
    +\big(8 \underset{\mp}{\omega}
    -\underset{\pm}{\omega} 
    -\underset{\mp}{\chi}\,_{ij} g^{ij}\big)\partial_\mp
    -\big(4 \underset{\mp}{\omega}
    +\underset{\pm}{\omega}
    +\underset{\pm}{\chi}\,_{ij} g^{ij} \big)\partial_\pm
    \Big) R_{\pm\pm}\\
    &\quad 
    + 2 R_{ij} \; \cdot \; \underset{\mp}{\chi}\,_{nm} \underset{\mp}{\chi}\,_{kl}g^{il}g^{jm}g^{kn}  \\
    &\quad 
    + 2 R_{\mp\pm} \; \cdot \; \underset{\mp}{\chi}\,_{jl} \underset{\mp}{\chi}\,_{ik} g^{kl} g^{ij} \\
    &\quad 
    + 2 R_{i\pm}  \; \cdot \;  \Big( + g^{jk}\big( \underset{\mp}{\chi}\,_{kl}\Gamma_{jm}^i g^{lm}
     -  \partial_j(\underset{\mp}{\chi}\,_{kl}g^{il})
    -  \underset{\mp}{\eta}\,_j \Gamma_{\pm k}^i\big)
    + \partial_\pm(\underset{\mp}{\eta}\,_j g^{ij})
    + \big(\underset{\pm}{\omega} \underset{\mp}{\eta}\,_j 
    -3 \underset{\mp}{\omega} \underset{\mp}{\eta}\,_j \big)g^{ij}\\
    &\quad \quad \quad \quad \quad \quad \;
     +  (\underset{\mp}{\chi}\,_{kl} \underset{\mp}{\chi}\,_{jk}
     +  \underset{\mp}{\chi}\,_{jk} \underset{\mp}{\eta}\,_l
     \pm  \zeta_j \underset{\mp}{\chi}\,_{kl}
     \pm  2 \zeta_k \underset{\mp}{\chi}\,_{jl}
     +  \Gamma_{jk}^m \underset{\mp}{\chi}\,_{ml}
     -  \underset{\pm}{\eta}\,_j\underset{_\mp}{\chi}\,_{kl}
     - \underset{\mp}{\eta}\,_j\underset{_\mp}{\chi}\,_{kl}
     )g^{il} g^{jk}\Big)\\
    &\quad 
    +4 g^{ij} \big( \underset{\mp}{\eta}\,_j \partial_\pm - \underset{\mp}{\chi}\,_{kj} g^{kl} \partial_l \big) R_{i \pm}
\end{align*}

We apologies for not writing it explicitly, for it is far too big an expression, but from \color{red} previous equations \color{black} we conclude that:
\begin{equation}
    \boxed{C_{\pm\pm} = (2\alpha + \beta + 2\gamma) A_{\pm\pm} +(4\gamma- \beta)B_{\pm\pm} + \mathcal{O}(R^2)}
\end{equation}
\end{document}